Add `Config`

Stlc/Basic.lean
@@ -1,19 +1,37 @@
 namespace Stlc
 
+structure Config : Type where
+  hasBool : Bool
+deriving DecidableEq
+
+namespace Config
+
+class HasBool (c : Config) : Prop where
+  hasBool : c.hasBool
+deriving DecidableEq
+
+instance : HasBool { hasBool := true } :=
+  { hasBool := rfl }
+
+end Config
+
+instance : DecidablePred Config.HasBool := fun c ↦
+  decidable_of_bool c.hasBool ⟨fun h ↦ { hasBool := h }, fun h ↦ h.hasBool⟩
+
 def TermVar : Type := String
 deriving DecidableEq
 
-inductive Ty : Type
-| bool
-| arrow : Ty → Ty → Ty
+inductive Ty (c : Config) : Type
+| bool [c.HasBool] : Ty c
+| arrow : Ty c → Ty c → Ty c
 deriving DecidableEq
 
-inductive Term : Type
-| var : TermVar → Term
-| abs : TermVar → Ty → Term → Term
-| app : Term → Term → Term
-| bool : Bool → Term
-| ite : Term → Term → Term → Term
+inductive Term (c : Config) : Type
+| var : TermVar → Term c
+| abs : TermVar → Ty c → Term c → Term c
+| app : Term c → Term c → Term c
+| bool [c.HasBool] : Bool → Term c
+| ite [c.HasBool] : Term c → Term c → Term c → Term c
 deriving DecidableEq
 
 end Stlc
