Stlc/Value.lean
@@ -3,28 +3,30 @@ import Stlc.Syntax
 
 namespace Stlc.Term
 
+variable {c : Config}
+
 open Syntax
 
 @[mk_iff]
-inductive Value : Term → Prop
+inductive Value : Term c → Prop
 | abs {x τ t} : Value t[λ x : τ, t]
-| bool {b} : Value (.bool b)
+| bool {b} [c.HasBool] : Value (bool b)
 
 attribute [simp] Value.abs Value.bool
 
 @[simp]
-lemma Value.var_not {x : TermVar} : ¬Value t[xⱽ] := by
+lemma Value.var_not {x : TermVar} : ¬@Value c t[xⱽ] := by
   rintro ⟨⟩
 
 @[simp]
-lemma Value.app_not {t₁ t₂ : Term} : ¬Value t[t₁ t₂] := by
+lemma Value.app_not {t₁ t₂ : Term c} : ¬Value t[t₁ t₂] := by
   rintro ⟨⟩
 
 @[simp]
-lemma Value.ite_not {t₁ t₂ t₃ : Term} : ¬Value t[if t₁ then t₂ else t₃] := by
+lemma Value.ite_not {t₁ t₂ t₃ : Term c} [c.HasBool] : ¬Value t[if t₁ then t₂ else t₃] := by
   rintro ⟨⟩
 
-instance : DecidablePred Value := fun t ↦
-  decidable_of_bool (t matches .bool _ | .abs ..) (by cases t <;> simp)
+instance : DecidablePred (@Value c) := fun t ↦
+  decidable_of_bool (t matches bool _ | abs ..) (by cases t <;> simp)
 
 end Stlc.Term
